user 5, session 19, part 36

diffs-annotated-fixed/5/user-5-session-19.v
@@ -140,14 +140,74 @@ apply <- evalEqTrue in IHt2.
 (rewrite H in IHt1).
 (rewrite IHt1 in IHt2).
 symmetry.
-(apply evalEqTrue).
+apply -> evalEqTrue.
 assumption.
 +
 (rewrite H).
 (apply evalEqFalse in H).
 (assert (eval L env (identity t1) <> eval L env (identity t2)) by congruence).
 symmetry.
-(apply evalEqFalse).
+apply -> evalEqFalse.
 assumption.
+Admitted.
+Fixpoint free_vars (t : Term) : list Identifier :=
+  match t with
+  | Var x => [x]
+  | Int _ => []
+  | Bool _ => []
+  | Eq a b => free_vars a ++ free_vars b
+  | And a b => free_vars a ++ free_vars b
+  | Or a b => free_vars a ++ free_vars b
+  | Not a => free_vars a
+  | If a b c => free_vars a ++ free_vars b ++ free_vars c
+  | Plus a b => free_vars a ++ free_vars b
+  | Times a b => free_vars a ++ free_vars b
+  | Minus a b => free_vars a ++ free_vars b
+  | Choose x P =>
+      filter (fun y => if id_eq_dec x y then false else true) (free_vars P)
+  end.
+Axiom (fresh_var : list Identifier -> Identifier).
+Axiom (fresh_var_unique : forall exclude, ~ In (fresh_var exclude) exclude).
+Definition Divide (t1 : Term) (t2 : Term) :=
+  let x := fresh_var (free_vars t1 ++ free_vars t2) in
+  Choose x (Eq t1 (Times (Var x) t2)).
+Lemma extendEnv_eq :
+  forall Value env x (val : Value), (extendEnv env x val) x = val.
+Admitted.
+Lemma divide_test :
+  forall L env, L.(eval) env (Divide (Int 6) (Int 2)) = L.(eval) env (Int 3).
+Proof.
+(intros).
+(unfold Divide).
+(match goal with
+ | |- context [ Choose ?x _ ] => generalize x
+ end).
+intro x.
+(assert
+  (forall res,
+   eval L env (Choose x (Eq (Int 6) (Times (Var x) (Int 2)))) = res ->
+   res = eval L env (Int 3))).
+{
+(intros).
+(assert
+  (eval L
+     (extendEnv env x
+        (eval L env (Choose x (Eq (Int 6) (Times (Var x) (Int 2))))))
+     (Eq (Int 6) (Times (Var x) (Int 2))) = L.(vTrue))).
+{
+(apply evalChoose).
+exists (eval L env (Int 3)).
+(apply evalEqTrue).
+(rewrite evalTimes with (i := 3%Z) (j := 2%Z)).
+-
+reflexivity.
+-
+(rewrite evalVar).
+(rewrite extendEnv_eq).
+(apply evalIntConst).
+-
+reflexivity.
+}
+admit.
 (* Auto-generated comment: Succeeded. *)
 
